proved base case

coq/two/LambdaTwo.v
@@ -1,7 +1,8 @@
 Require Export LambdaTwoSyntax.
 Require Export IndistinguishabilityTwo.
+Require Import LibTactics.
 
-Function eval (L : two) (P : value -> value -> Prop) (pc : two) (e : env)
+Fixpoint eval (L : two) (P : value -> value -> Prop) (pc : two) (e : env)
          (t : term) (k : nat) (a : atom) {struct k} :=
   match t with
     | TNat n =>
@@ -12,9 +13,9 @@ Function eval (L : two) (P : value -> value -> Prop) (pc : two) (e : env)
           a = Atom v (l ⊔ pc)
         | None => False
       end
-    | TLam t' =>
+    | TAbs t' =>
       a = Atom (VClos e t') pc
-    (*| TApp t1 t2 =>
+    | TApp t1 t2 =>
       match k with
         | S k' =>
           forall e1' t1' l1 a2 a3,
@@ -23,8 +24,8 @@ Function eval (L : two) (P : value -> value -> Prop) (pc : two) (e : env)
             eval L P l1 (a2 :: e1') t1' k' a3 ->
             a = a3
         | 0 => False
-      end*)
-    (*| TDecl t1 t2 =>
+      end
+    | TDecl t1 t2 =>
       match k with
         | S k' =>
           forall e1' t1' l1 a2 v3 l3,
@@ -33,15 +34,68 @@ Function eval (L : two) (P : value -> value -> Prop) (pc : two) (e : env)
             eval L P l1 (a2 :: e1') t1' k' (Atom v3 l3) ->
             match l3 with
               | Bottom2 =>
-                a = (Atom v3 Bottom2)
+                a = Atom v3 Bottom2
               | Top2 =>
                 (forall a2' e2' v3',
                    env_LPequiv L P (a2 :: e1') (a2' :: e2') ->
                    eval L P l1 (a2' :: e2') t1' k' (Atom v3' Top2) ->
                    value_LPequiv L P v3 v3') ->
-                a = (Atom v3 Bottom2)
+                a = Atom v3 Bottom2
             end
         | 0 => False
-      end*)
-    | _ => False
+      end
   end.
+
+Lemma eval_nat_inv :
+  forall L P k pc e n a,
+    eval L P pc e (TNat n) k a ->
+    a = Atom (VNat n) pc.
+Proof.
+  introv Heval.
+  destruct k; auto.
+Qed.
+
+Lemma eval_var_inv :
+  forall L P k pc e n v l a,
+    eval L P pc e (TVar n) k a ->
+    a = Atom v l ->
+    (l = Bottom2 /\
+     atIndex e n = Some (Atom v Bottom2)) \/
+    (l = Top2 /\ pc = Top2 /\
+     atIndex e n = Some (Atom v Bottom2)) \/
+    (l = Top2 /\ pc = Top2 /\
+     atIndex e n = Some (Atom v Top2)) \/
+    (l = Top2 /\ pc = Bottom2 /\
+     atIndex e n = Some (Atom v Top2)).
+Proof.
+  introv Heval Ha.
+  destruct l; destruct pc; subst.
+  - destruct k; unfold eval in Heval;
+    remember (atIndex e n) as o; destruct o as [[v' l'] |]; subst; auto;
+    rewrite join_bot in Heval; inversion Heval;
+    left; auto.
+  - destruct k; unfold eval in Heval;
+    remember (atIndex e n) as o; destruct o as [[v' l'] |]; subst; auto;
+    rewrite join_top in Heval; inversion Heval; 
+    left; auto.
+  - destruct k; unfold eval in Heval;
+    remember (atIndex e n) as o; destruct o as [[v' l'] |]; subst; auto;
+    rewrite join_bot in Heval; inversion Heval;
+    right; right; right; auto.
+  - destruct k; unfold eval in Heval;
+    remember (atIndex e n) as o; destruct o as [[v' l'] |]; subst; auto;
+    inversion Heval; destruct l'.
+    + right. left. auto.
+    + right. right. left. auto.
+    + right. left. auto.
+    + right. right. left. auto.
+Qed.
+
+Lemma eval_abs_inv :
+  forall L P k pc e t a,
+    eval L P pc e (TAbs t) k a ->
+    a = Atom (VClos e t) pc.
+Proof.
+  introv Heval.
+  destruct k; auto.
+Qed.
