coq/two/LambdaTwoNI.v
@@ -1,7 +1,82 @@
 Require Import Program.Tactics.
 Require Import LambdaTwo.
+Require Import LibTactics.
 
 Section NI.
+
+Lemma non_interference_nat :
+  forall L P k pc e1 e2 t a1 a2,
+    forall n,
+      t = TNat n ->
+      env_LPequiv L P e1 e2 ->
+      eval L P pc e1 t k a1 ->
+      eval L P pc e2 t k a2 ->
+      (forall x, P x x) ->
+      atom_LPequiv L P a1 a2.
+Proof.
+  introv Ht He Heval1 Heval2 Prefl. subst.
+  assert (Ha1: a1 = (Atom (VNat n) pc)) by (eapply eval_nat_inv; eauto).
+  assert (Ha2: a2 = (Atom (VNat n) pc)) by (eapply eval_nat_inv; eauto).
+  destruct L; destruct pc; subst.
+  - right. left. auto.
+  - left. auto.
+  - right. right. auto.
+  - right. right. auto.
+Qed.
+
+Lemma non_interference_var :
+  forall L P k pc e1 e2 t a1 a2,
+    forall n,
+      t = TVar n ->
+      env_LPequiv L P e1 e2 ->
+      eval L P pc e1 t k a1 ->
+      eval L P pc e2 t k a2 ->
+      (forall x, P x x) ->
+      atom_LPequiv L P a1 a2.
+Proof.
+  introv Ht He Heval1 Heval2 Prefl. subst.
+  remember (atIndex e1 n) as o1.
+  remember (atIndex e2 n) as o2.
+  destruct o1 as [[v1 l1] |];
+  destruct o2 as [[v2 l2] |].
+  - assert (atom_LPequiv L P (Atom v1 l1) (Atom v2 l2)) by
+        (eapply list_forall2_atIndex; eauto).
+    assert (l2 = l1) by
+        (apply atom_LPequiv_lab_inv in H; auto). subst.
+    destruct k; unfold eval in Heval1; unfold eval in Heval2;
+    repeat (rewrite <- Heqo1 in Heval1; rewrite <- Heqo2 in Heval2; subst;
+            destruct pc; [
+              rewrite join_bot; assumption |
+              rewrite join_top; destruct l1; try assumption;
+              apply atom_LPequiv_raise; auto
+           ]).
+  - destruct k; unfold eval in Heval2;
+    rewrite <- Heqo2 in Heval2; inversion Heval2.
+  - destruct k; unfold eval in Heval1;
+    rewrite <- Heqo1 in Heval1; inversion Heval1.
+  - destruct k; unfold eval in Heval1;
+    rewrite <- Heqo1 in Heval1; inversion Heval1.
+Qed.
+
+Lemma non_interference_abs :
+  forall L P k pc e1 e2 t a1 a2,
+    forall t',
+      t = TAbs t' ->
+      env_LPequiv L P e1 e2 ->
+      eval L P pc e1 t k a1 ->
+      eval L P pc e2 t k a2 ->
+      (forall x, P x x) ->
+      atom_LPequiv L P a1 a2.
+Proof.
+  introv Ht He Heval1 Heval2 Prefl. subst.
+  assert (Ha1: a1 = (Atom (VClos e1 t') pc)) by (eapply eval_abs_inv; eauto).
+  assert (Ha2: a2 = (Atom (VClos e2 t') pc)) by (eapply eval_abs_inv; eauto).
+  destruct L; destruct pc; subst.
+  - right. left. auto.
+  - left. auto.
+  - right. right. auto.
+  - right. right. auto.
+Qed.
 
 Theorem non_interference_strong_observer :
   forall L (P : value -> value -> Prop) k pc e1 e2 t a1 a2,
@@ -11,33 +86,7 @@ Theorem non_interference_strong_observer :
     eval L P pc e2 t k a2 -> 
     atom_LPequiv L P a1 a2.
 Proof.
-  intros L P k pc e1 e2 t a1 a2 Prefl He Heval1 Heval2.
-  generalize dependent a2.
-  generalize dependent e2.
-  functional induction (eval L P pc e1 t k a1);
-    simpl; auto; intros; subst.
-  - (* E_Nat *)
-    destruct L; destruct pc.
-    + right. left. auto.
-    + left. auto.
-    + right. right. auto.
-    + right. right. auto.
-  - (* E_Var *)
-    remember (atIndex e2 n) as o2. destruct o2 as [[v' l'] |].
-    + assert (atom_LPequiv L P (Atom v l) (Atom v' l')) by
-          (eapply list_forall2_atIndex; eauto).
-      assert (l' = l) by
-          (destruct H; destruct H; destruct_conjs; subst; auto).
-      destruct pc; destruct l; subst; auto.
-      apply atom_LPequiv_raise; auto.
-    + inversion Heval2.
-  - (* E_Abs *)
-    destruct L; destruct pc.
-    + right. left. auto.
-    + left. auto.
-    + right. right. auto.
-    + right. right. auto.
-Qed.
+  Admitted.
 
 Theorem non_interference :
   forall L (P : value -> value -> Prop) k pc e1 e2 t a1 a2,
